code/bignum/Hacl.Bignum.GenericField.fst
@@ -1,0 +1,135 @@
+module Hacl.Bignum.GenericField
+
+open FStar.HyperStack
+open FStar.HyperStack.ST
+open FStar.Mul
+
+open Lib.IntTypes
+open Lib.Buffer
+
+open Hacl.Bignum.Definitions
+
+module B = LowStar.Buffer
+module HS = FStar.HyperStack
+module ST = FStar.HyperStack.ST
+
+module Euclid = FStar.Math.Euclid
+module S = Hacl.Spec.Bignum.GenericField
+module BE = Hacl.Bignum.Exponentiation
+module IE = Hacl.Impl.Exponentiation
+module BN = Hacl.Bignum
+module BM = Hacl.Bignum.Montgomery
+
+friend Hacl.Bignum.Exponentiation
+friend Hacl.Spec.Bignum.GenericField
+
+#set-options "--z3rlimit 50 --fuel 1 --ifuel 0"
+
+let bn_field_get_len k _ =
+  k.len
+
+
+let bn_field_init km r nBits n =
+  [@inline_let]
+  let len = km.BM.bn.BN.len in
+  let h0 = ST.get () in
+  let r2 : buffer (limb U64) = LowStar.Monotonic.Buffer.mmalloc r (uint #U64 #SEC 0) len in
+  let n1 : buffer (limb U64) = LowStar.Monotonic.Buffer.mmalloc r (uint #U64 #SEC 0) len in
+  let h1 = ST.get () in
+  B.(modifies_only_not_unused_in loc_none h0 h1);
+  assert (B.length r2 == FStar.UInt32.v len);
+  assert (B.length n1 == FStar.UInt32.v len);
+  let r2 : lbignum U64 len = r2 in
+  let n1 : lbignum U64 len = n1 in
+  copy n1 n;
+
+  km.BM.precomp (nBits -! 1ul) n r2;
+  let mu = BM.mod_inv_limb n.(0ul) in
+  let res : bn_mont_ctx = { nBits = nBits; len = len; n = n1; mu = mu; r2 = r2 } in
+  let h2 = ST.get () in
+  assert (as_ctx h2 res == S.bn_field_init (v nBits) (as_seq h0 n));
+  assert (S.bn_mont_ctx_inv (as_ctx h2 res));
+  B.(modifies_only_not_unused_in loc_none h0 h2);
+  res
+
+
+let bn_to_field km k a aM =
+  let h0 = ST.get () in
+  km.BM.to k.n k.mu k.r2 a aM;
+  let h1 = ST.get () in
+  assert (as_seq h1 aM == S.bn_to_field (as_ctx h0 k) (as_seq h0 a));
+  assert (bn_v h1 aM < bn_v h0 k.n)
+
+
+let bn_from_field km k aM a =
+  let h0 = ST.get () in
+  km.BM.from k.n k.mu aM a;
+  let h1 = ST.get () in
+  assert (as_seq h1 a == S.bn_from_field (as_ctx h0 k) (as_seq h0 aM));
+  assert (bn_v h1 a < bn_v h0 k.n)
+
+
+let bn_field_add km k aM bM cM =
+  let h0 = ST.get () in
+  km.BM.bn.BN.add_mod_n k.n aM bM cM;
+  let h1 = ST.get () in
+  assert (as_seq h1 cM == S.bn_field_add (as_ctx h0 k) (as_seq h0 aM) (as_seq h0 bM));
+  assert (bn_v h1 cM < bn_v h0 k.n)
+
+
+let bn_field_sub km k aM bM cM =
+  let h0 = ST.get () in
+  BN.bn_sub_mod_n k.len k.n aM bM cM;
+  let h1 = ST.get () in
+  assert (as_seq h1 cM == S.bn_field_sub (as_ctx h0 k) (as_seq h0 aM) (as_seq h0 bM));
+  assert (bn_v h1 cM < bn_v h0 k.n)
+
+
+let bn_field_mul km k aM bM cM =
+  let h0 = ST.get () in
+  km.BM.mul k.n k.mu aM bM cM;
+  let h1 = ST.get () in
+  assert (as_seq h1 cM == S.bn_field_mul (as_ctx h0 k) (as_seq h0 aM) (as_seq h0 bM));
+  assert (bn_v h1 cM < bn_v h0 k.n)
+
+
+let bn_field_sqr km k aM cM =
+  let h0 = ST.get () in
+  km.BM.sqr k.n k.mu aM cM;
+  let h1 = ST.get () in
+  assert (as_seq h1 cM == S.bn_field_sqr (as_ctx h0 k) (as_seq h0 aM));
+  assert (bn_v h1 cM < bn_v h0 k.n)
+
+
+let bn_field_one km k oneM =
+  let h0 = ST.get () in
+  BM.bn_mont_one km k.n k.mu k.r2 oneM;
+  let h1 = ST.get () in
+  assert (as_seq h1 oneM == S.bn_field_one (as_ctx h0 k));
+  assert (bn_v h1 oneM < bn_v h0 k.n)
+
+
+let bn_field_inv km k aM aInvM =
+  [@inline_let]
+  let len = k.len in
+  push_frame ();
+  let n2 = create len (uint #U64 #SEC 0) in
+  let c = BN.bn_sub1 len k.n (uint #U64 #SEC 2) n2 in
+  let h0 = ST.get () in
+  S.bn_field_inv_lemma (as_ctx h0 k) (as_seq h0 aM);
+  Hacl.Spec.Bignum.bn_sub1_lemma (as_seq h0 k.n) (uint #U64 #SEC 2);
+  Hacl.Spec.Bignum.Definitions.bn_eval_bound (as_seq h0 n2) (v len);
+  Hacl.Spec.Bignum.Definitions.bn_eval_bound (as_seq h0 k.n) (v len);
+  BE.bn_mont_one km k.n k.mu k.r2 aInvM;
+  IE.lexp_fw_vartime len len (BE.mk_lexp U64 km ((as_ctx h0 k).S.n) k.mu) k.n aM len k.nBits n2 aInvM 4ul;
+  let h1 = ST.get () in
+  assert (bn_v h0 n2 == bn_v h0 k.n - 2);
+  assert (as_seq h1 aInvM ==
+    Lib.Exponentiation.exp_fw
+    (Hacl.Spec.Bignum.Exponentiation.mk_bn_mont_comm_monoid ((as_ctx h0 k).S.n) k.mu)
+    (as_seq h0 aM) (v k.nBits) (bn_v h0 k.n - 2) 4);
+
+  norm_spec [delta_only [`%S.bn_field_inv]] (S.bn_field_inv (as_ctx h0 k) (as_seq h0 aM));
+  assert (as_seq h1 aInvM == S.bn_field_inv (as_ctx h0 k) (as_seq h0 aM));
+  assert (bn_v h1 aInvM < bn_v h0 k.n);
+  pop_frame ()
