code/bignum/Hacl.Bignum.GenericField.fsti
@@ -1,0 +1,230 @@
+module Hacl.Bignum.GenericField
+
+open FStar.HyperStack
+open FStar.HyperStack.ST
+open FStar.Mul
+
+open Lib.IntTypes
+open Lib.Buffer
+
+open Hacl.Bignum.Definitions
+
+module B = LowStar.Buffer
+module HS = FStar.HyperStack
+module ST = FStar.HyperStack.ST
+
+module Euclid = FStar.Math.Euclid
+module S = Hacl.Spec.Bignum.GenericField
+module BE = Hacl.Bignum.Exponentiation
+module BN = Hacl.Bignum
+module BM = Hacl.Bignum.Montgomery
+
+#set-options "--z3rlimit 50 --fuel 0 --ifuel 0"
+
+//inline_for_extraction noextract
+class bn_mont_ctx = {
+  nBits: size_t;
+  len: BN.meta_len U64;
+  n: lbignum U64 len;
+  mu: limb U64;
+  r2: lbignum U64 len;
+  }
+
+
+inline_for_extraction noextract
+let as_ctx (h:mem) (k:bn_mont_ctx) : GTot (S.bn_mont_ctx U64) = {
+  S.nBits = v k.nBits;
+  S.len = v k.len;
+  S.n = as_seq h k.n;
+  S.mu = k.mu;
+  S.r2 = as_seq h k.r2;
+  }
+
+
+inline_for_extraction noextract
+let bn_mont_ctx_inv (h:mem) (k:bn_mont_ctx) =
+  live h k.n /\ live h k.r2 /\ disjoint k.n k.r2 /\
+  S.bn_mont_ctx_inv (as_ctx h k)
+
+
+inline_for_extraction noextract
+let bn_field_get_len_st (k:bn_mont_ctx) = unit ->
+  Stack (BN.meta_len U64)
+  (requires fun h -> bn_mont_ctx_inv h k)
+  (ensures  fun h0 r h1 -> h0 == h1 /\
+    v r == S.bn_field_get_len (as_ctx h0 k))
+
+
+inline_for_extraction noextract
+val bn_field_get_len: k:bn_mont_ctx -> bn_field_get_len_st k
+
+
+inline_for_extraction noextract
+let bn_field_init_st (len:BN.meta_len U64) =
+    r:HS.rid
+  -> nBits:size_t
+  -> n:lbignum U64 len ->
+  ST (bn_mont_ctx)
+  (requires fun h ->
+    live h n /\ S.bn_mont_ctx_pre (v nBits) (v len) (as_seq h n) /\
+    ST.is_eternal_region r)
+  (ensures  fun h0 res h1 ->
+    B.(modifies loc_none h0 h1) /\
+    S.bn_mont_ctx_inv (as_ctx h1 res) /\
+    B.(fresh_loc (loc_union (loc_buffer (res.n <: buffer (limb U64))) (loc_buffer (res.r2 <: buffer (limb U64)))) h0 h1) /\
+    B.(loc_includes (loc_region_only false r) (loc_union (loc_buffer (res.n <: buffer (limb U64))) (loc_buffer (res.r2 <: buffer (limb U64))))) /\
+    as_ctx h1 res == S.bn_field_init (v nBits) (as_seq h0 n))
+
+
+inline_for_extraction noextract
+val bn_field_init: km:BM.mont U64 -> bn_field_init_st km.BM.bn.BN.len
+
+
+inline_for_extraction noextract
+let bn_to_field_st (k:bn_mont_ctx) =
+    a:lbignum U64 k.len
+  -> aM:lbignum U64 k.len ->
+  Stack unit
+  (requires fun h ->
+    bn_mont_ctx_inv h k /\ live h a /\ live h aM /\ disjoint a aM /\
+    disjoint a k.r2 /\ disjoint a k.n /\
+    disjoint aM k.r2 /\ disjoint aM k.n /\
+    bn_v h a < bn_v h k.n)
+  (ensures  fun h0 _ h1 -> modifies (loc aM) h0 h1 /\
+    bn_v h1 aM < bn_v h0 k.n /\
+    as_seq h1 aM == S.bn_to_field (as_ctx h0 k) (as_seq h0 a))
+
+
+inline_for_extraction noextract
+val bn_to_field: km:BM.mont U64 -> k:bn_mont_ctx{k.len == km.BM.bn.BN.len} -> bn_to_field_st k
+
+
+inline_for_extraction noextract
+let bn_from_field_st (k:bn_mont_ctx) =
+    aM:lbignum U64 k.len
+  -> a:lbignum U64 k.len ->
+  Stack unit
+  (requires fun h ->
+    bn_mont_ctx_inv h k /\ live h a /\ live h aM /\ disjoint a aM /\
+    disjoint a k.r2 /\ disjoint a k.n /\
+    disjoint aM k.r2 /\ disjoint aM k.n /\
+    bn_v h aM < bn_v h k.n)
+  (ensures  fun h0 _ h1 -> modifies (loc a) h0 h1 /\
+    bn_v h1 a < bn_v h0 k.n /\
+    as_seq h1 a == S.bn_from_field (as_ctx h0 k) (as_seq h0 aM))
+
+
+inline_for_extraction noextract
+val bn_from_field: km:BM.mont U64 -> k:bn_mont_ctx{k.len == km.BM.bn.BN.len} -> bn_from_field_st k
+
+
+inline_for_extraction noextract
+let bn_field_add_st (k:bn_mont_ctx) =
+    aM:lbignum U64 k.len
+  -> bM:lbignum U64 k.len
+  -> cM:lbignum U64 k.len ->
+  Stack unit
+  (requires fun h ->
+    bn_mont_ctx_inv h k /\ live h aM /\ live h bM /\ live h cM /\
+    eq_or_disjoint aM bM /\ eq_or_disjoint aM cM /\ eq_or_disjoint bM cM /\
+    disjoint k.n aM /\ disjoint k.n bM /\ disjoint k.n cM /\
+    bn_v h aM < bn_v h k.n /\ bn_v h bM < bn_v h k.n)
+  (ensures  fun h0 _ h1 -> modifies (loc cM) h0 h1 /\
+    bn_v h1 cM < bn_v h0 k.n /\
+    as_seq h1 cM == S.bn_field_add (as_ctx h0 k) (as_seq h0 aM) (as_seq h0 bM))
+
+
+inline_for_extraction noextract
+val bn_field_add: km:BM.mont U64 -> k:bn_mont_ctx{k.len == km.BM.bn.BN.len} -> bn_field_add_st k
+
+
+inline_for_extraction noextract
+let bn_field_sub_st (k:bn_mont_ctx) =
+    aM:lbignum U64 k.len
+  -> bM:lbignum U64 k.len
+  -> cM:lbignum U64 k.len ->
+  Stack unit
+  (requires fun h ->
+    bn_mont_ctx_inv h k /\ live h aM /\ live h bM /\ live h cM /\
+    eq_or_disjoint aM bM /\ eq_or_disjoint aM cM /\ eq_or_disjoint bM cM /\
+    disjoint k.n aM /\ disjoint k.n bM /\ disjoint k.n cM /\
+    bn_v h aM < bn_v h k.n /\ bn_v h bM < bn_v h k.n)
+  (ensures  fun h0 _ h1 -> modifies (loc cM) h0 h1 /\
+    bn_v h1 cM < bn_v h0 k.n /\
+    as_seq h1 cM == S.bn_field_sub (as_ctx h0 k) (as_seq h0 aM) (as_seq h0 bM))
+
+
+inline_for_extraction noextract
+val bn_field_sub: km:BM.mont U64 -> k:bn_mont_ctx{k.len == km.BM.bn.BN.len} -> bn_field_sub_st k
+
+
+inline_for_extraction noextract
+let bn_field_mul_st (k:bn_mont_ctx) =
+    aM:lbignum U64 k.len
+  -> bM:lbignum U64 k.len
+  -> cM:lbignum U64 k.len ->
+  Stack unit
+  (requires fun h ->
+    bn_mont_ctx_inv h k /\ live h aM /\ live h bM /\ live h cM /\
+    eq_or_disjoint aM bM /\ eq_or_disjoint aM cM /\ eq_or_disjoint bM cM /\
+    disjoint cM k.n /\
+    bn_v h aM < bn_v h k.n /\ bn_v h bM < bn_v h k.n)
+  (ensures  fun h0 _ h1 -> modifies (loc cM) h0 h1 /\
+    bn_v h1 cM < bn_v h0 k.n /\
+    as_seq h1 cM == S.bn_field_mul (as_ctx h0 k) (as_seq h0 aM) (as_seq h0 bM))
+
+
+inline_for_extraction noextract
+val bn_field_mul: km:BM.mont U64 -> k:bn_mont_ctx{k.len == km.BM.bn.BN.len} -> bn_field_mul_st k
+
+
+inline_for_extraction noextract
+let bn_field_sqr_st (k:bn_mont_ctx) =
+    aM:lbignum U64 k.len
+  -> cM:lbignum U64 k.len ->
+  Stack unit
+  (requires fun h ->
+    bn_mont_ctx_inv h k /\ live h aM /\ live h cM /\
+    eq_or_disjoint aM cM /\ disjoint cM k.n /\
+    bn_v h aM < bn_v h k.n)
+  (ensures  fun h0 _ h1 -> modifies (loc cM) h0 h1 /\
+    bn_v h1 cM < bn_v h0 k.n /\
+    as_seq h1 cM == S.bn_field_sqr (as_ctx h0 k) (as_seq h0 aM))
+
+
+inline_for_extraction noextract
+val bn_field_sqr: km:BM.mont U64 -> k:bn_mont_ctx{k.len == km.BM.bn.BN.len} -> bn_field_sqr_st k
+
+
+inline_for_extraction noextract
+let bn_field_one_st (k:bn_mont_ctx) = oneM:lbignum U64 k.len ->
+  Stack unit
+  (requires fun h ->
+    bn_mont_ctx_inv h k /\ live h oneM /\
+    disjoint k.n oneM /\ disjoint k.r2 oneM)
+  (ensures  fun h0 _ h1 -> modifies (loc oneM) h0 h1 /\
+    bn_v h1 oneM < bn_v h0 k.n /\
+    as_seq h1 oneM == S.bn_field_one (as_ctx h0 k))
+
+
+inline_for_extraction noextract
+val bn_field_one: km:BM.mont U64 -> k:bn_mont_ctx{k.len == km.BM.bn.BN.len} -> bn_field_one_st k
+
+
+inline_for_extraction noextract
+let bn_field_inv_st (k:bn_mont_ctx) =
+    aM:lbignum U64 k.len
+  -> aInvM:lbignum U64 k.len ->
+  Stack unit
+  (requires fun h ->
+    bn_mont_ctx_inv h k /\ live h aM /\ live h aInvM /\
+    disjoint aM aInvM /\ disjoint k.n aM /\
+    disjoint k.n aInvM /\ disjoint k.r2 aInvM /\
+    0 < bn_v h aM /\ bn_v h aM < bn_v h k.n)
+  (ensures  fun h0 _ h1 -> modifies (loc aInvM) h0 h1 /\
+    bn_v h1 aInvM < bn_v h0 k.n /\
+    as_seq h1 aInvM == S.bn_field_inv (as_ctx h0 k) (as_seq h0 aM))
+
+
+inline_for_extraction noextract
+val bn_field_inv: km:BM.mont U64 -> k:bn_mont_ctx{k.len == km.BM.bn.BN.len} -> bn_field_inv_st k
