code/bignum/Hacl.GenericField64.fst
@@ -1,0 +1,43 @@
+module Hacl.GenericField64
+
+open FStar.Mul
+
+module BN = Hacl.Bignum
+module GF = Hacl.Bignum.GenericField
+module BM = Hacl.Bignum.Montgomery
+
+#set-options "--z3rlimit 50 --fuel 0 --ifuel 0"
+
+inline_for_extraction noextract
+let km (len:BN.meta_len Lib.IntTypes.U64) =
+  BM.mk_runtime_mont len
+
+let field_init len r nBits n =
+  GF.bn_field_init (km len) r nBits n
+
+let field_get_len k =
+  GF.bn_field_get_len k
+
+let to_field k a aM =
+  GF.bn_to_field (km k.GF.len) k a aM
+
+let from_field k aM a =
+  GF.bn_from_field (km k.GF.len) k aM a
+
+let add k aM bM cM =
+  GF.bn_field_add (km k.GF.len) k aM bM cM
+
+let sub k aM bM cM =
+  GF.bn_field_sub (km k.GF.len) k aM bM cM
+
+let mul k aM bM cM =
+  GF.bn_field_mul (km k.GF.len) k aM bM cM
+
+let sqr k aM cM =
+  GF.bn_field_sqr (km k.GF.len) k aM cM
+
+let one k oneM =
+  GF.bn_field_one (km k.GF.len) k oneM
+
+let inverse k aM aInvM =
+  GF.bn_field_inv (km k.GF.len) k aM aInvM
