code/bignum/Hacl.GenericField64.fsti
@@ -1,0 +1,128 @@
+module Hacl.GenericField64
+
+open FStar.Mul
+
+module BN = Hacl.Bignum
+module GF = Hacl.Bignum.GenericField
+
+#set-options "--z3rlimit 50 --fuel 0 --ifuel 0"
+
+[@@ CPrologue
+"/*******************************************************************************
+
+A verified field arithmetic library.
+
+This is a 64-bit optimized version, where bignums are represented as an array
+of `len` unsigned 64-bit integers, i.e. uint64_t[len].
+All the arithmetic operations are performed in the Montgomery domen.
+
+*******************************************************************************/\n";
+Comment "Allocate and initialize a montgomery context.
+
+  The argument n is meant to be `len` limbs in size, i.e. uint64_t[len].
+  The argument nBits is an exact number of significant bits of n.
+
+  This function is *UNSAFE* and requires C clients to observe bn_mont_ctx_pre
+  from Hacl.Spec.Bignum.GenericField.fsti, which amounts to:
+
+  • 0 < nBits /\ (nBits - 1) / bits t < len
+  • pow2 (nBits - 1) < n /\ n < pow2 nBits
+
+  • n % 2 = 1
+  • 1 < n
+
+  • n is a prime // needed for the modular multiplicative inverse
+"]
+val field_init: len:BN.meta_len Lib.IntTypes.U64 -> GF.bn_field_init_st len
+
+[@@ Comment "Return a size of the modulus `n` in limbs.
+
+  The argument k is a montgomery context obtained through Hacl_GenericField64_field_init."]
+val field_get_len: k:GF.bn_mont_ctx -> GF.bn_field_get_len_st k
+
+[@@ Comment "Convert a bignum to its Montgomery representation.
+
+  Write `a * R mod n` in `aM`.
+
+  The arguments a and aM are meant to be `len` limbs in size, i.e. uint64_t[len].
+  The argument k is a montgomery context obtained through Hacl_GenericField64_field_init.
+
+  This function is *UNSAFE* and requires C clients to observe bn_to_field
+  from Hacl.Spec.Bignum.GenericField.fsti, which amounts to:
+  • a < n
+"]
+val to_field: k:GF.bn_mont_ctx -> GF.bn_to_field_st k
+
+[@@ Comment "Convert the result back from the Montgomery representation to the regular representation.
+
+  Write `aM / R mod n` in `a`, i.e.
+  Hacl_GenericField64_from_field(k, Hacl_GenericField64_to_field(k, a)) == a
+
+  The arguments a and aM are meant to be `len` limbs in size, i.e. uint64_t[len].
+  The argument k is a montgomery context obtained through Hacl_GenericField64_field_init.
+
+  This function is *UNSAFE* and requires C clients to observe bn_from_field
+  from Hacl.Spec.Bignum.GenericField.fsti, which amounts to:
+  • aM < n
+"]
+val from_field: k:GF.bn_mont_ctx -> GF.bn_from_field_st k
+
+[@@ Comment "Write `aM + bM mod n` in `cM`.
+
+  The arguments aM, bM, and cM are meant to be `len` limbs in size, i.e. uint64_t[len].
+  The argument k is a montgomery context obtained through Hacl_GenericField64_field_init.
+
+  This function is *UNSAFE* and requires C clients to observe bn_field_add
+  from Hacl.Spec.Bignum.GenericField.fsti, which amounts to:
+  • aM < n
+  • bM < n "]
+val add: k:GF.bn_mont_ctx -> GF.bn_field_add_st k
+
+[@@ Comment "Write `aM - bM mod n` to `cM`.
+
+  The arguments aM, bM, and cM are meant to be `len` limbs in size, i.e. uint64_t[len].
+  The argument k is a montgomery context obtained through Hacl_GenericField64_field_init.
+
+  This function is *UNSAFE* and requires C clients to observe bn_field_sub
+  from Hacl.Spec.Bignum.GenericField.fsti, which amounts to:
+  • aM < n
+  • bM < n "]
+val sub: k:GF.bn_mont_ctx -> GF.bn_field_sub_st k
+
+[@@ Comment "Write `aM * bM mod n` in `cM`.
+
+  The arguments aM, bM, and cM are meant to be `len` limbs in size, i.e. uint64_t[len].
+  The argument k is a montgomery context obtained through Hacl_GenericField64_field_init.
+
+  This function is *UNSAFE* and requires C clients to observe bn_field_mul
+  from Hacl.Spec.Bignum.GenericField.fsti, which amounts to:
+  • aM < n
+  • bM < n "]
+val mul: k:GF.bn_mont_ctx -> GF.bn_field_mul_st k
+
+[@@ Comment "Write `aM * aM mod n` in `cM`.
+
+  The arguments aM and cM are meant to be `len` limbs in size, i.e. uint64_t[len].
+  The argument k is a montgomery context obtained through Hacl_GenericField64_field_init.
+
+  This function is *UNSAFE* and requires C clients to observe bn_field_sqr
+  from Hacl.Spec.Bignum.GenericField.fsti, which amounts to:
+  • aM < n "]
+val sqr: k:GF.bn_mont_ctx -> GF.bn_field_sqr_st k
+
+[@@ Comment "Convert a bignum `one` to its Montgomery representation.
+
+  The argument oneM is meant to be `len` limbs in size, i.e. uint64_t[len].
+  The argument k is a montgomery context obtained through Hacl_GenericField64_field_init."]
+val one: k:GF.bn_mont_ctx -> GF.bn_field_one_st k
+
+[@@ Comment "Write `aM ^ (-1) mod n` in `aInvM`.
+
+  The arguments aM and aInvM are meant to be `len` limbs in size, i.e. uint64_t[len].
+  The argument k is a montgomery context obtained through Hacl_GenericField64_field_init.
+
+  This function is *UNSAFE* and requires C clients to observe bn_field_inv
+  from Hacl.Spec.Bignum.GenericField.fsti, which amounts to:
+  • aM < n
+  • 0 < aM "]
+val inverse: k:GF.bn_mont_ctx -> GF.bn_field_inv_st k
