code/bignum/Hacl.Spec.Bignum.GenericField.fst
@@ -1,0 +1,414 @@
+module Hacl.Spec.Bignum.GenericField
+
+open FStar.Mul
+
+open Lib.IntTypes
+open Lib.Sequence
+
+open Hacl.Spec.Bignum.Definitions
+
+module Euclid = FStar.Math.Euclid
+module LE = Lib.Exponentiation
+module M = Hacl.Spec.Montgomery.Lemmas
+module E = Hacl.Spec.Exponentiation.Lemmas
+module BE = Hacl.Spec.Bignum.Exponentiation
+module BM = Hacl.Spec.Bignum.Montgomery
+module BN = Hacl.Spec.Bignum
+module BB = Hacl.Spec.Bignum.Base
+module BIL = Hacl.Spec.Bignum.ModInvLimb
+module BI = Hacl.Spec.Bignum.ModInv
+
+
+friend Hacl.Spec.Bignum.Exponentiation
+
+#set-options "--z3rlimit 50 --fuel 0 --ifuel 0"
+
+//////////////////////////////////////////
+
+val mul_zero_lemma: n:pos{Euclid.is_prime n} -> x:int -> y:int ->
+  Lemma (x * y % n == 0 <==> (x % n == 0 \/ y % n == 0))
+let mul_zero_lemma n x y =
+  if x % n = 0 then
+    Math.Lemmas.lemma_mod_mul_distr_l x y n
+  else
+    if y % n = 0 then
+      Math.Lemmas.lemma_mod_mul_distr_r x y n
+    else
+      if x * y % n = 0 then
+        Math.Fermat.mod_mult_congr n x 0 y
+      else ()
+
+
+val mul_nonzero_lemma: n:pos{Euclid.is_prime n} -> x:int -> y:int -> Lemma
+  (requires x % n <> 0 /\ y % n <> 0)
+  (ensures  x * y % n <> 0)
+let mul_nonzero_lemma n x y =
+  mul_zero_lemma n x y
+
+
+val from_mont_add_lemma: #t:limb_t -> k:bn_mont_ctx t{bn_mont_ctx_inv k} -> aM:lbignum t k.len -> bM:lbignum t k.len -> Lemma
+  (requires bn_v aM < bn_v k.n /\ bn_v bM < bn_v k.n)
+  (ensures
+   (let cM = (bn_v aM + bn_v bM) % bn_v k.n in
+    let c = M.from_mont (bits t) k.len (bn_v k.n) (v k.mu) cM in
+    let a = M.from_mont (bits t) k.len (bn_v k.n) (v k.mu) (bn_v aM) in
+    let b = M.from_mont (bits t) k.len (bn_v k.n) (v k.mu) (bn_v bM) in
+    c == (a + b) % bn_v k.n))
+
+let from_mont_add_lemma #t k aM bM =
+  let r = pow2 (bits t * k.len) in
+  let d, _ = M.eea_pow2_odd (bits t * k.len) (bn_v k.n) in
+  bn_eval_bound k.n k.len;
+  M.mont_preconditions (bits t) k.len (bn_v k.n) (v k.mu);
+  assert (r * d % bn_v k.n == 1 /\ bn_v k.n < r /\ (1 + bn_v k.n * v k.mu) % pow2 (bits t) == 0);
+
+  let cM = (bn_v aM + bn_v bM) % bn_v k.n in
+  let c = M.from_mont (bits t) k.len (bn_v k.n) (v k.mu) cM in
+  let a = M.from_mont (bits t) k.len (bn_v k.n) (v k.mu) (bn_v aM) in
+  let b = M.from_mont (bits t) k.len (bn_v k.n) (v k.mu) (bn_v bM) in
+
+  M.from_mont_lemma (bits t) k.len (bn_v k.n) d (v k.mu) cM;
+  assert (c == cM * d % bn_v k.n);
+
+  calc (==) { //c
+    cM * d % bn_v k.n;
+    (==) { }
+    (bn_v aM + bn_v bM) % bn_v k.n * d % bn_v k.n;
+    (==) { Math.Lemmas.lemma_mod_mul_distr_l (bn_v aM + bn_v bM) d (bn_v k.n) }
+    (bn_v aM + bn_v bM) * d % bn_v k.n;
+    (==) { Math.Lemmas.distributivity_add_left (bn_v aM) (bn_v bM) d }
+    (bn_v aM * d + bn_v bM * d) % bn_v k.n;
+    (==) { Math.Lemmas.modulo_distributivity (bn_v aM * d) (bn_v bM * d) (bn_v k.n) }
+    (bn_v aM * d % bn_v k.n + bn_v bM * d % bn_v k.n) % bn_v k.n;
+    };
+
+  M.from_mont_lemma (bits t) k.len (bn_v k.n) d (v k.mu) (bn_v aM);
+  M.from_mont_lemma (bits t) k.len (bn_v k.n) d (v k.mu) (bn_v bM)
+
+
+val from_mont_sub_lemma: #t:limb_t -> k:bn_mont_ctx t{bn_mont_ctx_inv k} -> aM:lbignum t k.len -> bM:lbignum t k.len -> Lemma
+  (requires bn_v aM < bn_v k.n /\ bn_v bM < bn_v k.n)
+  (ensures
+   (let cM = (bn_v aM - bn_v bM) % bn_v k.n in
+    let c = M.from_mont (bits t) k.len (bn_v k.n) (v k.mu) cM in
+    let a = M.from_mont (bits t) k.len (bn_v k.n) (v k.mu) (bn_v aM) in
+    let b = M.from_mont (bits t) k.len (bn_v k.n) (v k.mu) (bn_v bM) in
+    c == (a - b) % bn_v k.n))
+
+let from_mont_sub_lemma #t k aM bM =
+  let r = pow2 (bits t * k.len) in
+  let d, _ = M.eea_pow2_odd (bits t * k.len) (bn_v k.n) in
+  bn_eval_bound k.n k.len;
+  M.mont_preconditions (bits t) k.len (bn_v k.n) (v k.mu);
+  assert (r * d % bn_v k.n == 1 /\ bn_v k.n < r /\ (1 + bn_v k.n * v k.mu) % pow2 (bits t) == 0);
+
+  let cM = (bn_v aM - bn_v bM) % bn_v k.n in
+  let c = M.from_mont (bits t) k.len (bn_v k.n) (v k.mu) cM in
+  let a = M.from_mont (bits t) k.len (bn_v k.n) (v k.mu) (bn_v aM) in
+  let b = M.from_mont (bits t) k.len (bn_v k.n) (v k.mu) (bn_v bM) in
+
+  M.from_mont_lemma (bits t) k.len (bn_v k.n) d (v k.mu) cM;
+  assert (c == cM * d % bn_v k.n);
+
+  calc (==) { //c
+    cM * d % bn_v k.n;
+    (==) { }
+    (bn_v aM - bn_v bM) % bn_v k.n * d % bn_v k.n;
+    (==) { Math.Lemmas.lemma_mod_mul_distr_l (bn_v aM - bn_v bM) d (bn_v k.n) }
+    (bn_v aM - bn_v bM) * d % bn_v k.n;
+    (==) { Math.Lemmas.distributivity_sub_left (bn_v aM) (bn_v bM) d }
+    (bn_v aM * d - bn_v bM * d) % bn_v k.n;
+    (==) { Math.Lemmas.lemma_mod_plus_distr_l (bn_v aM * d) (- bn_v bM * d) (bn_v k.n) }
+    (bn_v aM * d % bn_v k.n - bn_v bM * d) % bn_v k.n;
+    (==) { Math.Lemmas.lemma_mod_sub_distr (bn_v aM * d % bn_v k.n) (bn_v bM * d) (bn_v k.n) }
+    (bn_v aM * d % bn_v k.n - bn_v bM * d % bn_v k.n) % bn_v k.n;
+    };
+
+  M.from_mont_lemma (bits t) k.len (bn_v k.n) d (v k.mu) (bn_v aM);
+  M.from_mont_lemma (bits t) k.len (bn_v k.n) d (v k.mu) (bn_v bM)
+
+
+val from_mont_mul_lemma: #t:limb_t -> k:bn_mont_ctx t{bn_mont_ctx_inv k} -> aM:lbignum t k.len -> bM:lbignum t k.len -> Lemma
+  (requires bn_v aM < bn_v k.n /\ bn_v bM < bn_v k.n)
+  (ensures
+   (let cM = M.mont_mul (bits t) k.len (bn_v k.n) (v k.mu) (bn_v aM) (bn_v bM) in
+    let c = M.from_mont (bits t) k.len (bn_v k.n) (v k.mu) cM in
+    let a = M.from_mont (bits t) k.len (bn_v k.n) (v k.mu) (bn_v aM) in
+    let b = M.from_mont (bits t) k.len (bn_v k.n) (v k.mu) (bn_v bM) in
+    c == a * b % bn_v k.n))
+
+let from_mont_mul_lemma #t k aM bM =
+  let r = pow2 (bits t * k.len) in
+  let d, _ = M.eea_pow2_odd (bits t * k.len) (bn_v k.n) in
+  bn_eval_bound k.n k.len;
+  M.mont_preconditions (bits t) k.len (bn_v k.n) (v k.mu);
+  assert (r * d % bn_v k.n == 1 /\ bn_v k.n < r /\ (1 + bn_v k.n * v k.mu) % pow2 (bits t) == 0);
+
+  let cM = M.mont_mul (bits t) k.len (bn_v k.n) (v k.mu) (bn_v aM) (bn_v bM) in
+  let c = M.from_mont (bits t) k.len (bn_v k.n) (v k.mu) cM in
+  let a = M.from_mont (bits t) k.len (bn_v k.n) (v k.mu) (bn_v aM) in
+  let b = M.from_mont (bits t) k.len (bn_v k.n) (v k.mu) (bn_v bM) in
+
+  M.mont_mul_lemma (bits t) k.len (bn_v k.n) d (v k.mu) (bn_v aM) (bn_v bM);
+  assert (cM == bn_v aM * bn_v bM * d % bn_v k.n);
+
+  M.from_mont_lemma (bits t) k.len (bn_v k.n) d (v k.mu) cM;
+
+  calc (==) { //c
+    cM * d % bn_v k.n;
+    (==) { }
+    (bn_v aM * bn_v bM * d % bn_v k.n) * d % bn_v k.n;
+    (==) { Math.Lemmas.lemma_mod_mul_distr_l (bn_v aM * bn_v bM * d) d (bn_v k.n) }
+    bn_v aM * bn_v bM * d * d % bn_v k.n;
+    (==) { Math.Lemmas.paren_mul_right (bn_v aM) (bn_v bM) d }
+    bn_v aM * (bn_v bM * d) * d % bn_v k.n;
+    (==) {
+      Math.Lemmas.paren_mul_right (bn_v aM) (bn_v bM * d) d;
+      Math.Lemmas.swap_mul (bn_v bM * d) d;
+      Math.Lemmas.paren_mul_right (bn_v aM) d (bn_v bM * d) }
+    bn_v aM * d * (bn_v bM * d) % bn_v k.n;
+    (==) { Math.Lemmas.lemma_mod_mul_distr_l (bn_v aM * d) (bn_v bM * d) (bn_v k.n) }
+    (bn_v aM * d % bn_v k.n) * (bn_v bM * d) % bn_v k.n;
+    (==) { Math.Lemmas.lemma_mod_mul_distr_r (bn_v aM * d % bn_v k.n) (bn_v bM * d) (bn_v k.n) }
+    (bn_v aM * d % bn_v k.n) * (bn_v bM * d % bn_v k.n) % bn_v k.n;
+    };
+
+  M.from_mont_lemma (bits t) k.len (bn_v k.n) d (v k.mu) (bn_v aM);
+  M.from_mont_lemma (bits t) k.len (bn_v k.n) d (v k.mu) (bn_v bM)
+
+
+val from_mont_one_lemma: #t:limb_t -> k:bn_mont_ctx t{bn_mont_ctx_inv k} -> Lemma
+   (let oneM = M.mont_one (bits t) k.len (bn_v k.n) (v k.mu) in
+    let one = M.from_mont (bits t) k.len (bn_v k.n) (v k.mu) oneM in
+    one == 1)
+
+let from_mont_one_lemma #t k =
+  let r = pow2 (bits t * k.len) in
+  let d, _ = M.eea_pow2_odd (bits t * k.len) (bn_v k.n) in
+  bn_eval_bound k.n k.len;
+  M.mont_preconditions (bits t) k.len (bn_v k.n) (v k.mu);
+  assert (r * d % bn_v k.n == 1 /\ bn_v k.n < r /\ (1 + bn_v k.n * v k.mu) % pow2 (bits t) == 0);
+
+  let oneM = M.mont_one (bits t) k.len (bn_v k.n) (v k.mu) in
+  M.mont_one_lemma (bits t) k.len (bn_v k.n) d (v k.mu);
+  assert (oneM == r % bn_v k.n);
+  let one = M.from_mont (bits t) k.len (bn_v k.n) (v k.mu) oneM in
+  M.from_mont_lemma (bits t) k.len (bn_v k.n) d (v k.mu) oneM;
+  assert (one == oneM * d % bn_v k.n);
+  assert (one == (r % bn_v k.n) * d % bn_v k.n);
+  M.lemma_mont_id (bn_v k.n) r d 1;
+  assert (one == 1 % bn_v k.n);
+  Math.Lemmas.small_mod 1 (bn_v k.n)
+
+
+val from_mont_exp_lemma: #t:limb_t -> k:bn_mont_ctx t{bn_mont_ctx_inv k} -> aM:lbignum t k.len -> b:pos -> Lemma
+  (requires bn_v aM < bn_v k.n)
+  (ensures
+   (let cM = LE.pow (BE.mk_bn_mont_comm_monoid k.n k.mu) aM b in
+    let c = M.from_mont (bits t) k.len (bn_v k.n) (v k.mu) (bn_v cM) in
+    let a = M.from_mont (bits t) k.len (bn_v k.n) (v k.mu) (bn_v aM) in
+    c == Lib.NatMod.pow a b % bn_v k.n))
+
+let from_mont_exp_lemma #t k aM b =
+  let ke = BE.mk_bn_mont_comm_monoid k.n k.mu in
+  let cM = LE.pow ke aM b in
+  BE.lemma_bn_mont_pre_is_mont_pre k.n k.mu;
+  BE.pow_bn_mont_is_pow_nat_mont_ll k.n k.mu aM b;
+  assert (bn_v cM == LE.pow (E.mk_nat_mont_ll_comm_monoid (bits t) k.len (bn_v k.n) (v k.mu)) (bn_v aM) b);
+
+  let r = pow2 (bits t * k.len) in
+  let d, _ = M.eea_pow2_odd (bits t * k.len) (bn_v k.n) in
+  M.mont_preconditions_d (bits t) k.len (bn_v k.n);
+  E.pow_nat_mont_ll_is_pow_nat_mont (bits t) k.len (bn_v k.n) (v k.mu) (bn_v aM) b;
+  assert (bn_v cM == LE.pow (E.mk_nat_mont_comm_monoid (bn_v k.n) r d) (bn_v aM) b);
+  E.pow_nat_mont_is_pow (bn_v k.n) r d (bn_v aM) b;
+  assert (bn_v cM == Lib.NatMod.pow (bn_v aM) b * (1 * r % bn_v k.n) * Lib.NatMod.pow d b % bn_v k.n);
+
+  let tmp1 = Lib.NatMod.pow (bn_v aM) b in
+  let tmp2 = Lib.NatMod.pow d b in
+  let tmp3 = Lib.NatMod.pow (bn_v aM * d % bn_v k.n) b in
+
+  calc (==) { //cM
+    tmp1 * (1 * r % bn_v k.n) * tmp2 % bn_v k.n;
+    (==) {
+      Math.Lemmas.paren_mul_right tmp1 (1 * r % bn_v k.n) tmp2;
+      Math.Lemmas.swap_mul (1 * r % bn_v k.n) tmp2;
+      Math.Lemmas.paren_mul_right tmp1 tmp2 (1 * r % bn_v k.n) }
+    tmp1 * tmp2 * (1 * r % bn_v k.n) % bn_v k.n;
+    (==) { Math.Lemmas.lemma_mod_mul_distr_r (tmp1 * tmp2) (1 * r) (bn_v k.n) }
+    tmp1 * tmp2 * r % bn_v k.n;
+    (==) { Lib.NatMod.lemma_pow_mul_base (bn_v aM) d b }
+    Lib.NatMod.pow (bn_v aM * d) b * r % bn_v k.n;
+    (==) { Math.Lemmas.lemma_mod_mul_distr_l (Lib.NatMod.pow (bn_v aM * d) b) r (bn_v k.n) }
+    Lib.NatMod.pow (bn_v aM * d) b % bn_v k.n * r % bn_v k.n;
+    (==) { Lib.NatMod.lemma_pow_mod_base (bn_v aM * d) b (bn_v k.n) }
+    tmp3 % bn_v k.n * r % bn_v k.n;
+    (==) { Math.Lemmas.lemma_mod_mul_distr_l tmp3 r (bn_v k.n) }
+    tmp3 * r % bn_v k.n;
+    };
+
+  assert (bn_v cM == tmp3 * r % bn_v k.n);
+  let c = M.from_mont (bits t) k.len (bn_v k.n) (v k.mu) (bn_v cM) in
+  M.from_mont_lemma (bits t) k.len (bn_v k.n) d (v k.mu) (bn_v cM);
+  //assert (c == bn_v cM * d % bn_v k.n);
+  calc (==) { //c
+    bn_v cM * d % bn_v k.n;
+    (==) { }
+    tmp3 * r % bn_v k.n * d % bn_v k.n;
+    (==) { M.lemma_mont_id (bn_v k.n) r d tmp3 }
+    tmp3 % bn_v k.n;
+    };
+
+  M.from_mont_lemma (bits t) k.len (bn_v k.n) d (v k.mu) (bn_v aM)
+
+
+val from_mont_lemma_nonzero: #t:limb_t -> k:bn_mont_ctx t{bn_mont_ctx_inv k} -> aM:lbignum t k.len -> Lemma
+  (requires 0 < bn_v aM /\ bn_v aM < bn_v k.n)
+  (ensures
+   (let a = M.from_mont (bits t) k.len (bn_v k.n) (v k.mu) (bn_v aM) in
+    a <> 0 /\ a < bn_v k.n))
+
+let from_mont_lemma_nonzero #t k aM =
+  let r = pow2 (bits t * k.len) in
+  let d, k1 = M.eea_pow2_odd (bits t * k.len) (bn_v k.n) in
+  bn_eval_bound k.n k.len;
+  M.mont_preconditions (bits t) k.len (bn_v k.n) (v k.mu);
+
+  let a = M.from_mont (bits t) k.len (bn_v k.n) (v k.mu) (bn_v aM) in
+  M.from_mont_lemma (bits t) k.len (bn_v k.n) d (v k.mu) (bn_v aM);
+  assert (bn_v aM < bn_v k.n);
+  Math.Lemmas.small_mod (bn_v aM) (bn_v k.n);
+  assert (bn_v aM % bn_v k.n <> 0);
+
+  let d1 = -d in
+  assert (0 < d1 /\ d1 < bn_v k.n);
+  Math.Lemmas.lemma_mod_sub_1 d1 (bn_v k.n);
+  assert (d % bn_v k.n == bn_v k.n - (d1 % bn_v k.n));
+  assert (d % bn_v k.n <> 0);
+  mul_nonzero_lemma (bn_v k.n) (bn_v aM) d;
+  assert (bn_v aM * d % bn_v k.n <> 0)
+
+
+val bn_field_inv_lemma: #t:limb_t -> k:bn_mont_ctx t{bn_mont_ctx_inv k} -> aM:lbignum t k.len -> Lemma
+  (requires 0 < bn_v aM /\ bn_v aM < bn_v k.n)
+  (ensures (let n2 = bn_v k.n - 2 in
+    let ke = BE.mk_bn_mont_comm_monoid k.n k.mu in
+    let aInvM = LE.exp_fw ke aM k.nBits n2 4 in
+    let aInv = M.from_mont (bits t) k.len (bn_v k.n) (v k.mu) (bn_v aInvM) in
+    let a = M.from_mont (bits t) k.len (bn_v k.n) (v k.mu) (bn_v aM) in
+    aInv * a % bn_v k.n == 1))
+
+let bn_field_inv_lemma #t k aM =
+  let n2 = bn_v k.n - 2 in
+  let ke = BE.mk_bn_mont_comm_monoid k.n k.mu in
+  let accM = LE.exp_fw ke aM k.nBits n2 4 in
+  LE.exp_fw_lemma ke aM k.nBits n2 4;
+  assert (accM == LE.pow ke aM n2);
+  from_mont_exp_lemma #t k aM n2;
+
+  let acc = M.from_mont (bits t) k.len (bn_v k.n) (v k.mu) (bn_v accM) in
+  let a = M.from_mont (bits t) k.len (bn_v k.n) (v k.mu) (bn_v aM) in
+  from_mont_lemma_nonzero #t k aM;
+  assert (0 < a /\ a < bn_v k.n);
+  Lib.NatMod.lemma_pow_mod #(bn_v k.n) a n2;
+  assert (acc == Lib.NatMod.pow_mod #(bn_v k.n) a n2);
+  BI.mod_inv_prime_lemma (bn_v k.n) a;
+  assert (Lib.NatMod.pow_mod #(bn_v k.n) a n2 * a % bn_v k.n == 1)
+
+///////////////////////////////////////
+
+let bn_field_get_len #t k = k.len
+
+
+let bn_field_init #t #len nBits n =
+  BM.bn_precomp_r2_mod_n_lemma (nBits - 1) n;
+  let r2 = BM.bn_precomp_r2_mod_n (nBits - 1) n in
+  assert (bn_v r2 == pow2 (2 * bits t * len) % bn_v n);
+
+  let mu = BIL.mod_inv_limb n.[0] in
+  BIL.bn_mod_inv_limb_lemma n;
+  assert ((1 + (bn_v n % pow2 (bits t)) * v mu) % pow2 (bits t) == 0);
+
+  { nBits = nBits; len = len; n = n; mu = mu; r2 = r2 }
+
+
+let bn_to_field #t k a =
+  let aM = BM.bn_to_mont k.n k.mu k.r2 a in
+  BM.bn_to_mont_lemma k.n k.mu k.r2 a;
+  aM
+
+
+let bn_from_field #t k aM =
+  let a = BM.bn_from_mont k.n k.mu aM in
+  BM.bn_from_mont_lemma k.n k.mu aM;
+  a
+
+
+let bn_from_to_field_lemma #t k a =
+  let aM = bn_to_field k a in
+  let r = pow2 (bits t * k.len) in
+  let d, _ = M.eea_pow2_odd (bits t * k.len) (bn_v k.n) in
+  bn_eval_bound k.n k.len;
+  M.mont_preconditions (bits t) k.len (bn_v k.n) (v k.mu);
+  assert (r * d % bn_v k.n == 1 /\ bn_v k.n < r /\ (1 + bn_v k.n * v k.mu) % pow2 (bits t) == 0);
+
+  M.from_mont_lemma (bits t) k.len (bn_v k.n) d (v k.mu) (bn_v aM);
+  assert (bn_v (bn_from_field k aM) == bn_v aM * d % bn_v k.n);
+  M.to_mont_lemma (bits t) k.len (bn_v k.n) d (v k.mu) (bn_v a);
+  assert (bn_v aM == bn_v a * r % bn_v k.n);
+  M.lemma_mont_id (bn_v k.n) (pow2 (bits t * k.len)) d (bn_v a);
+  assert (bn_v (bn_from_field k aM) == bn_v a % bn_v k.n);
+  Math.Lemmas.small_mod (bn_v a) (bn_v k.n);
+  assert (bn_v (bn_from_field k aM) == bn_v a)
+
+
+let bn_field_add #t k aM bM =
+  let cM = BN.bn_add_mod_n k.n aM bM in
+  BN.bn_add_mod_n_lemma k.n aM bM;
+  assert (bn_v cM == (bn_v aM + bn_v bM) % bn_v k.n);
+  from_mont_add_lemma #t k aM bM;
+  cM
+
+
+let bn_field_sub #t k aM bM =
+  let cM = BN.bn_sub_mod_n k.n aM bM in
+  BN.bn_sub_mod_n_lemma k.n aM bM;
+  assert (bn_v cM == (bn_v aM - bn_v bM) % bn_v k.n);
+  from_mont_sub_lemma #t k aM bM;
+  cM
+
+
+let bn_field_mul #t k aM bM =
+  let cM = BM.bn_mont_mul k.n k.mu aM bM in
+  BM.bn_mont_mul_lemma k.n k.mu aM bM;
+  from_mont_mul_lemma #t k aM bM;
+  cM
+
+
+let bn_field_sqr #t k aM =
+  let cM = BM.bn_mont_sqr k.n k.mu aM in
+  BM.bn_mont_sqr_lemma k.n k.mu aM;
+  from_mont_mul_lemma #t k aM aM;
+  cM
+
+
+let bn_field_one #t k =
+  let oneM = BM.bn_mont_one k.n k.mu r2 in
+  BM.bn_mont_one_lemma k.n k.mu k.r2;
+  from_mont_one_lemma #t k;
+  oneM
+
+
+let bn_field_inv #t k aM =
+  let c, n2 = BN.bn_sub1 k.n (uint #t 2) in
+  BN.bn_sub1_lemma k.n (uint #t 2);
+  assert (bn_v n2 - v c * pow2 (bits t * k.len) == bn_v k.n - 2);
+  bn_eval_bound n2 k.len;
+  bn_eval_bound k.n k.len;
+  assert (v c = 0);
+  assert (bn_v n2 == bn_v k.n - 2);
+
+  bn_field_inv_lemma #t k aM;
+  let ke = BE.mk_bn_mont_comm_monoid k.n k.mu in
+  let aInvM = LE.exp_fw ke aM k.nBits (bn_v n2) 4 in
+  aInvM
